lntbr.v
@@ -46,18 +46,18 @@ rewrite dersrec_map_single ;
 rewrite -> Forall_map_single in acm ;
 rewrite -> ?can_gen_swapL_def' in acm ;
 rewrite -> ?can_gen_swapR_def' in acm ;
-unfold nslext.
+unfold nslclext ; unfold nslext.
 
 (* where exchange is in the first of two sequents of the modal rule *)
 Ltac use_acm1 acm rs := 
 (* interchange two sublists of list of formulae *)
 derIrs rs ; [> 
-apply NSlctxt2 ;
+apply NSlctxt2 || apply NSlclctxt2 ;
 assoc_single_mid ;
 apply WBoxLs || apply BBoxLs || apply WDiaRs || apply BDiaRs |
 ms_cgs acm ;
 list_assoc_r' ; simpl ; eapply acm ] ; [> | 
-  unfold nslext ; list_assoc_r' ; simpl ; reflexivity |
+  unfold nslext ; unfold nslclext ; list_assoc_r' ; simpl ; reflexivity |
   reflexivity ] ; 
 swap_tac.
 
@@ -65,13 +65,13 @@ swap_tac.
   in which conclusion has no principal formula *)
 Ltac use_acm2s acm rs rw :=
 derIrs rs ; [> 
-list_assoc_r' ; simpl ; apply NSlctxt2 ;
+list_assoc_r' ; simpl ; apply NSlctxt2 || apply NSlclctxt2 ;
 rw ; (* rewrite so as to identify two parts of context *)
 apply WBoxLs || apply BBoxLs || apply WDiaRs || apply BDiaRs |
 ms_cgs acm ;
 list_assoc_r' ; simpl ;
 rewrite list_rearr22 ; eapply acm ] ; [> | 
-  unfold nslext ; list_assoc_r' ; simpl ; reflexivity |
+  unfold nslext ; unfold nslclext ; list_assoc_r' ; simpl ; reflexivity |
   reflexivity ] ; swap_tac.
 
 Lemma gen_swapL_step_bsr: forall V ps concl last_rule rules,
@@ -159,13 +159,13 @@ Ltac use_acm_sw_sep acm rs swap :=
 (* interchange two sublists of list of formulae,
   no need to expand swap (swap separate from where rule is applied) *)
 derIrs rs ; [> 
-list_assoc_r' ; simpl ; apply NSlctxt2 ;
+list_assoc_r' ; simpl ; apply NSlclctxt2 || apply NSlctxt2 ;
 apply WBoxLs || apply BBoxLs || apply WDiaRs || apply BDiaRs |
 ms_cgs acm ;
 eapply acm in swap ] ;
 [> (rewrite - list_rearr21 ; eapply swap) || 
   (list_assoc_r' ; simpl ; eapply swap) |
-  unfold nslext ; list_assoc_r' ; simpl ; reflexivity |
+  unfold nslext ; unfold nslclext ; list_assoc_r' ; simpl ; reflexivity |
   reflexivity ].
 
 Lemma gen_swapR_step_bsr: forall V ps concl last_rule rules,
@@ -217,4 +217,114 @@ Check gen_swapR_step_bsr.
 (* for examples of how to combine these with other rules, 
   see lntmr.v, theorems gen_swapmsL and gen_swapmsR *)
 
-(* now want to do the same for left context only *)
+(* interchange two sublists of list of formulae,
+  no need to expand swap or the underlying rule *)
+
+(** now want to do the same for left context only **)
+Lemma gen_swapL_step_bsr_lc: forall V ps concl last_rule rules,
+  last_rule = nslclrule (@bsrules V) ->
+  gen_swapL_step last_rule rules ps concl.
+Proof.  intros until 0.  unfold gen_swapL_step.
+intros lreq nsr drs acm rs. clear drs. subst.
+
+inversion nsr as [? ? ? sppc mnsp nsc].
+unfold nslclext in nsc.
+rewrite can_gen_swapL_def'.  intros until 0. intros swap pp ss.
+unfold nslclext in pp. subst.
+
+acacD' ; subst ; rewrite -> ?app_nil_r in *. (* 3 subgoals, the various locs
+  where the exchange might be relative to where the rule is active *)
+
+(* swap in the first of the two sequents affected by the rule *)
+-{ clear nsr.  inversion sppc ; subst ; clear sppc. (* 2 subgoals *)
++{ inversion_clear swap. subst.
+  acacD' ; subst ; simpl ; rewrite ?app_nil_r ; (* 10 subgoals *)
+  use_acm1 acm rs. }
++{ inversion_clear swap. subst.
+  acacD' ; subst ; simpl ; rewrite ?app_nil_r ; (* 10 subgoals *)
+  use_acm1 acm rs. }
+  }
+
+(* case of exchange in sequent to the left of where rule applied *)
+-{ nsgen_sw nsr rs sppc c (Γ', Δ, d) acm inps0 swap. }
+
+(* here, swap in either of the two sequents affected by the rule *)
+-{ clear nsr.  inversion sppc ; subst ; clear sppc. (* 2 subgoals *)
+
+(* WBox *)
++{ acacD' ; subst ; simpl ; rewrite ?app_nil_r. (* 3 subgoals *)
+*{ inversion_clear swap. subst.
+  acacD' ; subst ; simpl ; rewrite ?app_nil_r ; (* 10 subgoals *)
+  use_acm1 acm rs. }
+(* swapping in second sequent of principal rule *) 
+*{
+inversion_clear swap. subst.
+acacD' ; subst.
+(* 4 subgoals, cases of where swapping occurs in the two parts
+  of context in conclusion (where no principal formula) *)
+{ use_acm2s acm rs ltac: (assoc_mid H1). }
+{ use_acm2s acm rs ltac: (assoc_mid H3). }
+{ use_acm2s acm rs list_assoc_l'. }
+{ use_acm2s acm rs ltac: (assoc_mid H). }
+}
+
+*{ list_eq_nc. contradiction. }
+}
+
+(* BBox *)
++{ acacD' ; subst ; simpl ; rewrite ?app_nil_r. (* 3 subgoals *)
+*{ inversion_clear swap. subst.
+  acacD' ; subst ; simpl ; rewrite ?app_nil_r ; (* 10 subgoals *)
+  use_acm1 acm rs. }
+(* swapping in second sequent of principal rule *) 
+*{
+inversion_clear swap. subst.
+acacD' ; subst.
+(* 4 subgoals, cases of where swapping occurs in the two parts
+  of context in conclusion (where no principal formula) *)
+{ use_acm2s acm rs ltac: (assoc_mid H1). }
+{ use_acm2s acm rs ltac: (assoc_mid H3). }
+{ use_acm2s acm rs list_assoc_l'. }
+{ use_acm2s acm rs ltac: (assoc_mid H). }
+}
+
+*{ list_eq_nc. contradiction. }
+}
+}
+Qed.
+
+Check gen_swapL_step_bsr_lc.
+
+Lemma gen_swapR_step_bsr_lc: forall V ps concl last_rule rules,
+  last_rule = nslclrule (@bsrules V) ->
+  gen_swapR_step last_rule rules ps concl.
+Proof.  intros until 0.  unfold gen_swapR_step.
+intros lreq nsr drs acm rs. clear drs. subst.
+
+inversion nsr as [? ? ? sppc mnsp nsc].
+unfold nslclext in nsc.
+rewrite can_gen_swapR_def'.  intros until 0. intros swap pp ss.
+unfold nslclext in pp. subst.
+
+acacD' ; subst ; rewrite -> ?app_nil_r in *. (* 3 subgoals, the various locs
+  where the exchange might be relative to where the rule is active *)
+
+-{ inversion sppc ; subst ; use_acm_sw_sep acm rs swap. }
+-{ nsgen_sw nsr rs sppc c (Γ, Δ', d) acm inps0 swap. }
+
+-{ clear nsr.  inversion sppc ; subst ; clear sppc. (* 2 subgoals *)
++{ acacD' ; subst ; simpl ; rewrite ?app_nil_r. (* 3 subgoals *)
+*{ use_acm_sw_sep acm rs swap. }
+*{ use_acm_sw_sep acm rs swap. }
+*{ list_eq_nc. contradiction. }
+}
++{ acacD' ; subst ; simpl ; rewrite ?app_nil_r. (* 3 subgoals *)
+*{ use_acm_sw_sep acm rs swap. }
+*{ use_acm_sw_sep acm rs swap. }
+*{ list_eq_nc. contradiction. }
+}
+}  
+
+Qed.
+
+Check gen_swapR_step_bsr_lc.
